chore: dang it, need to add meta code to build native_decide proof

SSA/Experimental/Bits/Fast/Tests.lean
@@ -23,13 +23,26 @@ theorem eq1 : ∀ (w : Nat) (a : BitVec w), a = a := by
 theorem eq2 (w : Nat) (a : BitVec w) : a = a := by
   bv_automata_gen (config := {backend := .circuit_cadical} )
 
-#eval Reflect.BvDecide.verifyAIG
+def lhs : Bool := Reflect.BvDecide.verifyAIG
       (Reflect.BvDecide.mkSafetyCircuit
           (predicateEvalEqFSM
               (Predicate.binary BinaryPredicate.eq ((Term.var 0).add (Term.var 1))
                 ((Term.var 1).add (Term.var 0)))).toFSM
           3).toAIG
       "3 0 1 2 0\n"
+
+theorem y : lhs = true := Lean.ofReduceBool _ _ rfl
+
+theorem x : Reflect.BvDecide.verifyAIG
+      (Reflect.BvDecide.mkSafetyCircuit
+          (predicateEvalEqFSM
+              (Predicate.binary BinaryPredicate.eq ((Term.var 0).add (Term.var 1))
+                ((Term.var 1).add (Term.var 0)))).toFSM
+          3).toAIG
+      "3 0 1 2 0\n" = true := y
+
+#print x._proof_1
+
 
 
 example (w : Nat) (a b : BitVec w) : a + b = b + a := by
